proof/Vector.v
@@ -1,115 +1,192 @@
 Require Import Coq.Arith.Arith.
-Parameter A : Set.
 
-Inductive vec : nat -> Set :=
-  | vnil : vec 0
-  | vcons : forall n, A -> vec n -> vec (S n).
+Section Vector.
+  Variable A : Set.
+  
+  Set Implicit Arguments.
 
-Definition hd : forall n, n > 0 -> vec n -> A.
-Proof.
-  intros n H v ; induction v.
-  elim (gt_irrefl _ H).
-  assumption.
-Defined.
+  Inductive vec : nat -> Set :=
+    | vnil : vec 0
+    | vcons : forall n, A -> vec n -> vec (S n).
+  
+  Definition hd : forall n, n > 0 -> vec n -> A.
+  Proof.
+    intros n H v ; induction v.
+    elim (gt_irrefl _ H).
+    assumption.
+  Defined.
+  
+  Definition tl : forall n, n > 0 -> vec n -> vec (pred n).
+  Proof.
+    intros n H v ; induction v.
+    elim (gt_irrefl _ H).
+    simpl.
+    assumption.
+  Defined.  
+  
+  
+  Lemma Sm_n_lt_m_n : forall n m, S n < m -> n < m.
+  Proof.
+    induction n ; simpl ; auto with arith.
+  Qed.
 
-Definition tl : forall n, n > 0 -> vec n -> vec (pred n).
-Proof.
-  intros n H v ; induction v.
-  elim (gt_irrefl _ H).
-  simpl.
-  assumption.
-Defined.  
+  Definition nth : forall n m, m < n -> vec n -> A.
+  Proof.
+    intros.
+    induction m.
+    induction H0.
+    elim (lt_n_O _ H).
+    assumption.
 
-Set Implicit Arguments.
+    apply IHm.
+    apply (Sm_n_lt_m_n H).
+  Defined.
 
-Definition nth : forall n m, m < n -> vec n -> A.
+  Require Import Omega.
+  
+  Definition vapp : forall n m, vec n -> vec m -> vec (n + m).
+  Proof.
+    intros.
+    induction H.
+    simpl.
+    assumption.
+    
+    pose (@vcons (n + m) a IHvec).
+    assert(S (n + m) = S n + m).
+    simpl.
+    reflexivity.
+    rewrite <- H1.
+    exact v.
+  Defined.
+
+  Require Import Eqdep.
+  
+  Definition vec_plus : forall n m, forall t : vec (n + m), 
+    exists t' : vec (m + n), eq_dep nat vec (n + m) t (m + n) t'.
+  Proof.
+    intros.
+    rewrite plus_comm.
+    exists t.
+    auto.
+  Qed.
+  
+  Require Import JMeq.
+
+  Lemma eq_dep_vnil : forall n, forall a : vec n,
+    n = 0 -> eq_dep nat vec n a 0 vnil.
+  Proof.
+    intros.
+    
+    simpl.
+    induction a.
+    auto.
+
+    discriminate.
+  Qed.
+
+  Lemma eq_vnil : forall v : vec 0, v = vnil.
+  Proof.
+    intros.
+    apply eq_dep_eq with (P := vec).
+    apply eq_dep_vnil.
+    auto.
+  Qed.
+
+  Lemma vapp_vnil_l : forall n, forall v : vec n,
+    vapp vnil v = v.
+  Proof.
+    intros.
+    simpl.
+    reflexivity.
+  Qed.
+
+  Lemma vapp_vnil_dep_l : forall n, forall v : vec n,
+    eq_dep nat vec n (vapp vnil v) n v.
+  Proof.
+    intros.
+    simpl.
+    apply eq_dep_intro.
+  Qed.
+  
+  Lemma vapp_vnil_dep_r : forall n, forall v : vec n,
+    eq_dep nat vec (n + 0) (vapp v vnil) n v.
+  Proof.
+    intros.
+    induction v.
+    simpl ; auto.
+
+    simpl.
+
+    pose (proj2 (equiv_eqex_eqdep nat vec (n + 0) n (vapp v vnil) v) IHv).
+    dependent rewrite -> e.
+    simpl.
+    auto.
+  Qed.
+End Vector.
+  
+Definition vmap : forall n, forall A B : Set, (A ->  B) -> vec A n -> vec B n.
 Proof.
   intros.
   induction H0.
-  elim (lt_n_O _ H).
-  assumption.
+  exact (vnil B).
+
+  exact (vcons (H a) IHvec).
 Defined.
+  
+Unset Implicit Arguments.
 
-Require Import Omega.
-
-Definition vapp : forall n m, vec n -> vec m -> vec (n + m).
+Lemma cons_nth : forall A : Set, forall i n, forall v : vec A n, forall a : A, forall p : i < n,
+  @nth A n i p v = @nth A (S n) (S i) (lt_n_S _ _ p) (vcons a v).
 Proof.
+  intros A i.
+  induction i.
   intros.
-  induction H.
+  unfold nth at 2.
   simpl.
-  assumption.
 
-  pose (vcons (n + m) a IHvec).
-  assert(S (n + m) = S n + m).
   simpl.
-  reflexivity.
-  rewrite <- H1.
-  exact v.
-Defined.
+  elim (lt_n_O _ p).
 
-Require Import Eqdep.
-
-Definition vec_plus : forall n m, forall t : vec (n + m), 
-  exists t' : vec (m + n), eq_dep nat vec (n + m) t (m + n) t'.
-Proof.
   intros.
-  rewrite plus_comm.
-  exists t.
-  auto.
-Qed.
-
-Require Import JMeq.
-
-Lemma eq_dep_vnil : forall n, forall a : vec n,
-  n = 0 -> eq_dep nat vec n a 0 vnil.
-Proof.
-  intros.
+  simpl.
+  simpl in IHn.
+  
   
   simpl.
-  induction a.
-  auto.
+  unfold nth ; simpl.
 
-  discriminate.
-Qed.
-
-Lemma eq_vnil : forall v : vec 0, v = vnil.
-Proof.
-  intros.
-  apply eq_dep_eq with (P := vec).
-  apply eq_dep_vnil.
-  auto.
-Qed.
-
-Lemma vapp_vnil_l : forall n, forall v : vec n,
-  vapp vnil v = v.
-Proof.
-  intros.
-  simpl.
-  reflexivity.
-Qed.
-
-Lemma vapp_vnil_dep_l : forall n, forall v : vec n,
-  eq_dep nat vec n (vapp vnil v) n v.
-Proof.
-  intros.
-  simpl.
-  apply eq_dep_intro.
-Qed.
+  simpl in IHn.
   
-Lemma vapp_vnil_dep_r : forall n, forall v : vec n,
-  eq_dep nat vec (n + 0) (vapp v vnil) n v.
-Proof.
-  intros.
+
+  assert(S i < n) ; try omega.
+
+  simpl in IHv.
+  simpl.
+  auto.
+
+  simpl.
+  simpl.
+  elim (lt_irrefl _ p).
+  pose (lt_asym _ _ p).
+  elim (n (lt_O_Sn i)).
+
+  simpl.
+  simpl in IHn.
   induction v.
-  simpl ; auto.
+  absurd (i < 0) ; try omega.
+  simpl.
+
+  
+  
+  
+  
+  simpl.
+  simpl in IHi.
+  
 
   simpl.
 
-  pose (proj2 (equiv_eqex_eqdep nat vec (n + 0) n (vapp v vnil) v) IHv).
-  dependent rewrite -> e.
-  simpl.
-  auto.
-Qed.
+
 
 Infix ":::" := vcons (at level 60, right associativity) : vector_scope.
 Infix "+++" := vapp (right associativity, at level 60) : vector_scope.
